src/goose_lang/ffi/jrnl_ffi.v
@@ -677,13 +677,13 @@ Proof.
   clear -Hstep Hctx.
   remember (e1, (s,g)) as ρ1 eqn:Hρ1.
   remember (e2, (jrnl_upd σj2 s,g)) as ρ2 eqn:Hρ2.
-  revert Hρ1 Hρ2.
+  revert Hρ1 Hρ2. destruct g.
   generalize (jrnl_upd σj2 s) as s'.
-  revert e1 e2 s g.
+  revert e1 e2 s.
   induction Hstep.
   - intros. rewrite Hρ1 in Hρ2. inversion Hρ2. subst.
     apply rtc_refl.
-  - intros. subst. destruct y as (e0'&s0'&g0').
+  - intros. subst. destruct y as (e0'&s0'&[]).
     eapply rtc_l; last first.
     { eapply IHHstep; eauto. }
     simpl. eapply fill_step'. eauto.
@@ -743,7 +743,7 @@ Proof.
     * rewrite ?dom_insert_L H2. set_solver.
     * apply wf_jrnl_extend; auto.
     * apply wf_jrnl_extend; auto. congruence.
-  - intros s Hsub_state.
+  - intros s g Hsub_state.
     rewrite insert_jrnl_upd //.
     rewrite {1}(insert_jrnl_sub_state _ _ _ _ Hsub_state).
     apply Hstep.
@@ -769,7 +769,7 @@ Lemma always_steps_lifting_puredet K `{Hctx: LanguageCtx' (ext := @spec_ext_op_f
                                              (ffi_semantics := (spec_ext_semantics_field))
                                              K}:
   ∀ e0 σ0 e1 σ1 e2,
-  (∀ σ, prim_step' e1 σ [] e2 σ []) →
+  (∀ σ g, prim_step' e1 σ g [] e2 σ g []) →
   always_steps e0 σ0 (K e1) σ1 →
   always_steps e0 σ0 (K e2) σ1.
 Proof.
@@ -777,9 +777,9 @@ Proof.
   split_and!; eauto.
   { eapply Hsteps. }
   { eapply Hsteps. }
-  intros s Hsub.
+  intros s g Hsub.
   destruct Hsteps as (?&?&Hrtc).
-  specialize (Hrtc _ Hsub).
+  specialize (Hrtc _ g Hsub).
   eapply rtc_r; eauto.
   simpl. eapply fill_step'. eapply Hdet.
 Qed.
@@ -799,16 +799,16 @@ Proof.
   intros Hwf Hlookup1 Hlookup2 Hk.
   split_and!; eauto.
   { split_and!; try set_solver. }
-  intros s Hsub.
+  intros s g Hsub.
   apply rtc_once.
-  eapply (Ectx_step' _ _ _ _ _ _ []) => //=.
+  eapply (Ectx_step' _ _ _ _ _ _ _ _ []) => //=.
   rewrite jrnl_upd_sub // /head_step//=.
   rewrite /jrnl_sub_state in Hsub.
   destruct Hsub as (?&Heq&?&?).
   destruct a as (ablk&aoff).
   econstructor; last econstructor; eauto.
   econstructor; repeat (econstructor; eauto).
-  { rewrite Heq. econstructor. eauto. }
+  { simpl. rewrite Heq. econstructor. eauto. }
   { simpl in Hlookup1.
     eapply lookup_weaken in Hlookup1; last eassumption.
     rewrite Hlookup1. econstructor; eauto. }
@@ -818,19 +818,19 @@ Proof.
   { rewrite /check/ifThenElse. rewrite decide_True //=. }
 Qed.
 
-Lemma ghost_step_open_stuck E j K {HCTX: LanguageCtx K} σ:
+Lemma ghost_step_open_stuck E j K {HCTX: LanguageCtx K} σ g:
   nclose sN_inv ⊆ E →
   (∀ vs, σ.(@world _ jrnl_spec_ffi_model.(@spec_ffi_model_field)) ≠ Closed vs) →
   j ⤇ K (ExternalOp (ext := @spec_ext_op_field jrnl_spec_ext) OpenOp #()) -∗
   source_ctx (CS := spec_crash_lang) -∗
-  source_state σ -∗
+  source_state σ g -∗
   |NC={E}=> False.
 Proof.
   iIntros (??) "Hj Hctx H".
   iMod (ghost_step_stuck with "Hj Hctx H") as "[]".
   { eapply stuck_ExternalOp; first (by eauto).
     apply head_irreducible_not_atomically; [ by inversion 1 | ].
-    intros ?????.
+    intros ??????.
     repeat (inv_head_step; simpl in *; repeat monad_inv).
     destruct (σ.(world)) eqn:Heq; try congruence;
     repeat (inv_head_step; simpl in *; repeat monad_inv); eauto.
@@ -846,7 +846,7 @@ Lemma jrnl_opened_open_false E j K {HCTX: LanguageCtx K}:
   False.
 Proof.
   iIntros (?) "(#Hctx&#Hstate) Hopened Hj".
-  iInv "Hstate" as (σ) "(>H&Hinterp)" "Hclo".
+  iInv "Hstate" as (σ g) "(>H&Hinterp)" "Hclo".
   iDestruct "Hinterp" as "(>Hσ&>Hffi&Hrest)".
   simpl.
   iDestruct (jrnl_ctx_unify_opened with "[$] [$]") as %Heq; subst.
@@ -863,7 +863,7 @@ Lemma jrnl_open_open_false E j K {HCTX: LanguageCtx K} j' K' {HCTX': LanguageCtx
   False.
 Proof.
   iIntros (?) "(#Hctx&#Hstate) Hj Hj'".
-  iInv "Hstate" as (σ) "(>H&Hinterp)" "Hclo".
+  iInv "Hstate" as (σ g) "(>H&Hinterp)" "Hclo".
   iDestruct "Hinterp" as "(>Hσ&>Hffi&Hrest)".
   iEval (simpl) in "Hffi".
   destruct σ.(world) eqn:Heq; rewrite Heq; try (iDestruct "Hffi" as %[]).
@@ -1123,15 +1123,15 @@ Lemma ghost_step_jrnl_atomically_abort E j K {HCTX: LanguageCtx K} (l: sval) e :
   j ⤇ K NONEV.
 Proof.
   iIntros (?) "(#Hctx&#Hstate) Hopen Hj".
-  iInv "Hstate" as (s) "(>H&Hinterp)" "Hclo".
+  iInv "Hstate" as (s g) "(>H&Hinterp)" "Hclo".
   iDestruct "Hinterp" as "(>Hσ&>Hffi&Hrest)".
   iMod (ghost_step_stuck' with "[$] [$] [$]") as (Hnstuck) "(Hj&H)"; first by solve_ndisj.
-  iMod (ghost_step_lifting _ _ _ _ _ [] _ _ [] with "[$] [$] [$]") as "($&Hstate'&_)".
+  iMod (ghost_step_lifting _ _ _ _ _ _ [] _ _ _ [] with "[$] [$] [$]") as "($&Hstate'&_)".
   { apply head_prim_step. eapply head_step_atomically_fail.
     eapply atomically_not_stuck_body_safe; eauto. }
   { solve_ndisj. }
   iMod ("Hclo" with "[-]") as "_".
-  { iNext. iExists _. iFrame. }
+  { iNext. iExists _, _. iFrame. }
   iModIntro. eauto.
 Qed.
 
@@ -1148,13 +1148,13 @@ Lemma ghost_step_jrnl_atomically E j K {HCTX: LanguageCtx K} (l: sval) e σj (v:
 Proof.
   iIntros (Hsteps ?) "(#Hctx&#Hstate) Hσj_data Hσj_kinds Hopen Hj".
   destruct Hsteps as (Heq_kinds&Hwf&Hrtc).
-  iInv "Hstate" as (s) "(>H&Hinterp)" "Hclo".
+  iInv "Hstate" as (s g) "(>H&Hinterp)" "Hclo".
   iDestruct "Hinterp" as "(>Hσ&>Hffi&Hrest)".
   iDestruct (jrnl_ctx_sub_state_valid with "[$] [$] [$] [$]") as %Hsub.
   iMod (ghost_step_stuck' with "[$] [$] [$]") as (Hnstuck) "(Hj&H)"; first by solve_ndisj.
-  iMod (ghost_step_lifting _ _ _ (Atomically l e) s [] (jrnl_upd σj' s) (SOMEV v) []
+  iMod (ghost_step_lifting _ _ _ (Atomically l e) s g [] (jrnl_upd σj' s) g (SOMEV v) []
           with "Hj Hctx H") as "(Hj&H&_)".
-  { apply head_prim_step.
+  { destruct g. apply head_prim_step.
     apply head_step_atomically; eauto.
     eapply atomically_not_stuck_body_safe; eauto.
   }
@@ -1163,7 +1163,7 @@ Proof.
   { destruct Hwf as (?&?&?&?). rewrite Heq_kinds; eauto. }
   { destruct Hwf as (?&?&?&?). eauto. }
   iMod ("Hclo" with "[Hσ Hrest H Hffi]") as "_".
-  { iNext. iExists _. iFrame "H". iFrame. }
+  { iNext. iExists _, _. iFrame "H". iFrame. }
   iModIntro. iFrame.
 Qed.
 
@@ -1200,13 +1200,13 @@ Proof.
     iDestruct (big_sepM_lookup_acc _ _ _ _ Hlookup with "Htok") as "(H1&_)"; eauto.
     iDestruct (ptsto_conflict with "[$] [$]") as %[].
   }
-  iDestruct "Hrest" as (s) "(>H&Hinterp)".
+  iDestruct "Hrest" as (s g) "(>H&Hinterp)".
   iDestruct "Hinterp" as "(>Hσ&>Hffi&?&?&?&>Hctok)".
   iDestruct (jrnl_ctx_sub_state_valid with "[$] [$] [$] [$]") as %Hsub.
   iIntros "#HC".
   iMod (ghost_step_crash_stuck' with "[] Hctx Hctok Hj [$] [$]") as (Hnstuck) "(Hj&H&Hctok)"; first by solve_ndisj.
   { iModIntro. iIntros "(h1&>h2)". iDestruct (pending_pending with "[$] [$]") as %[]. }
-  iMod (ghost_step_crash_lifting _ _ _ _ _ (Atomically l e) s [] (jrnl_upd σj' s) (SOMEV v) []
+  iMod (ghost_step_crash_lifting _ _ _ _ _ (Atomically l e) s g [] (jrnl_upd σj' s) g (SOMEV v) []
           with "[] Hctok Hj Hctx H HC") as "(Hctok&Hj&H&_)".
   { apply head_prim_step.
     apply head_step_atomically; eauto.
@@ -1218,14 +1218,14 @@ Proof.
   { destruct Hwf as (?&?&?&?). rewrite Heq_kinds; eauto. }
   { destruct Hwf as (?&?&?&?). eauto. }
   iMod ("Hclo" with "[-Hσj_crash_toks Hσj'_data]") as "_".
-  { iNext. iRight. iExists _. iFrame "H". iFrame. }
+  { iNext. iRight. iExists _, _. iFrame "H". iFrame. }
   iModIntro. iFrame.
 Qed.
 
 Lemma ghost_step_jrnl_atomically_ub E j K {HCTX: LanguageCtx K} (l: sval) e1 σj e2 σj' σdom :
-  (∀ s, jrnl_sub_state σj' s →
+  (∀ s g, jrnl_sub_state σj' s →
         dom (gset _) (jrnlData (get_jrnl s.(world))) = σdom →
-        stuck' e2 s) →
+        stuck' e2 s g) →
   always_steps e1 σj e2 σj' →
   nclose sN ⊆ E →
   spec_ctx -∗
@@ -1238,7 +1238,7 @@ Lemma ghost_step_jrnl_atomically_ub E j K {HCTX: LanguageCtx K} (l: sval) e1 σj
 Proof.
   iIntros (Hub Hsteps ?) "(#Hctx&#Hstate) Hσj_data Hσj_kinds Hdom Hopen Hj".
   destruct Hsteps as (Heq_kinds&Hwf&Hrtc).
-  iInv "Hstate" as (s) "(>H&Hinterp)" "Hclo".
+  iInv "Hstate" as (s g) "(>H&Hinterp)" "Hclo".
   iDestruct "Hinterp" as "(>Hσ&>Hffi&Hrest)".
   iDestruct (jrnl_ctx_sub_state_valid with "[$] [$] [$] [$]") as %Hsub.
   iDestruct (jrnl_ctx_dom_eq _ s with "[$] [$]") as %Hdom.
@@ -1251,14 +1251,14 @@ Proof.
     { move: Heq. destruct Ki => //=; congruence. }
     naive_solver.
   }
-  rewrite /irreducible. intros ???? Hnostep.
+  rewrite /irreducible. intros ????? Hnostep.
   inversion Hnostep; subst.
   {
     inversion H2; eauto.
   }
   {
     match goal with
-    | [ H: prim_step'_safe _ _ |- _ ] => eapply H; first eapply Hrtc; eauto
+    | [ H: prim_step'_safe _ _ _ |- _ ] => eapply H; first eapply Hrtc; eauto
     end.
     eapply Hub.
     { eapply jrnl_sub_state_upd; eauto. }
@@ -1274,7 +1274,7 @@ Proof.
   }
   {
     match goal with
-    | [ H: prim_step'_safe _ _ |- _ ] => eapply H; first eapply Hrtc; eauto
+    | [ H: prim_step'_safe _ _ _ |- _ ] => eapply H; first eapply Hrtc; eauto
     end.
     eapply Hub.
     { eapply jrnl_sub_state_upd; eauto. }
